change R to total mapping

coqimp/framework/logic/logic.v
@@ -26,6 +26,8 @@ Inductive asrt : Type :=
 | Aoexpevl : OpExp -> Word -> asrt
 | Areg : RegName -> Word -> asrt
 | Aregdly : nat -> SpReg -> Word -> asrt
+| ATimReduce : asrt -> asrt
+| Awin : asrt -> Frame -> Frame -> Frame -> asrt
 | Apure : Prop -> asrt
 | Aframe : Word -> FrameList -> asrt
 | Atrue : asrt
@@ -45,6 +47,8 @@ Notation "aexp '==ₓ' addr" := (Aaexpevl aexp addr) (at level 20).
 Notation "oexp '==ₑ' v" := (Aoexpevl oexp v) (at level 20).
 Notation "rn |=> v" := (Areg rn v) (at level 20).
 Notation "n '@' rn |==> v" := (Aregdly n rn v) (at level 20).
+Notation "'{[' p '#' fm1 , fm2 , fm3 ']}'" := (Awin p fm1 fm2 fm3) (at level 29).
+Notation "p ↓" := (ATimReduce p) (at level 28).
 
 Notation "'EX' x , p " :=
   (Aexists (fun x => p))
@@ -88,6 +92,16 @@ Definition getframelst (s : State) :=
   | (M, (R, F), D) => F
   end.
 
+Definition updregs (s : State) (R' : RegFile) :=
+  match s with
+  | (M, (R, F), D) => (M, (R', F), D)
+  end.
+
+Definition upddlyls (s : State) (D' : DelayList) :=
+  match s with
+  | (M, (R, F), D) => (M, (R, F), D')
+  end.
+
 Definition regInDlyBuff (rn : RegName) (D : DelayList) :=
   match rn with
   | Rr rr => False
@@ -121,7 +135,7 @@ Definition inDlyBuff (d : DelayItem) (D : DelayList) :=
 
 (* $ rn = v hold if the value v locates in memory with address R(rn) *)
 Definition regSt (rn : RegName) (v : Word) (s : State) :=
-  getregs s = RegMap.set rn (Some v) empR /\ getmem s = empM /\
+  (getregs s) rn = v /\ getmem s = empM /\
   ~ (regInDlyBuff rn (getdlyls s)).
 
 Fixpoint regdlySt (n : nat) (rsp : SpReg) (v : Word) (s : State) :=
@@ -135,31 +149,67 @@ and memory states and register state are disjoint *)
 Definition state_union (s1 s2 s : State) :=
   match s1, s2 with
   | (M1, (R1, F1), D1), (M2, (R2, F2), D2) =>
-    disjoint M1 M2 /\ disjoint R1 R2 /\
-    s = (merge M1 M2, (merge R1 R2, F1), D1) /\ F1 = F2 /\ D1 = D2
+    disjoint M1 M2 /\ s = (merge M1 M2, (R1, F1), D1) /\
+    R1 = R2 /\ F1 = F2 /\ D1 = D2
   end.
+
+(* the OpR describes a set registers mentioned in oexp  *)
+Definition OpR (oexp : OpExp) : list RegName :=
+  match oexp with
+  | Or rr => Rr rr :: nil
+  | Ow _ => nil
+  end.
+
+(* the ApR describes a set registers mentioned in aexp *)
+Definition ApR (aexp : AddrExp) : list RegName :=
+  match aexp with
+  | Ao oexp => OpR oexp
+  | Aro rr oexp => Rr rr :: OpR oexp
+  end.
+
+(* the operation FR whether register rn described in assertion p *)
+Fixpoint FR (rn : RegName) (p : asrt) {struct p} : Prop :=
+  match p with
+  | p //\\ q => FR rn p \/ FR rn q
+  | p \\// q => FR rn p \/ FR rn q
+  | p ** q => FR rn p \/ FR rn q
+  | Aforall t p => forall x : t, FR rn (p x)
+  | Aexists t p => forall x : t, FR rn (p x)
+  | p ↓ => FR rn p
+  | rn' |=> v => if RegNameEq.eq rn rn' then True else False
+  | t @ sr |==> v => if RegNameEq.eq rn (Rsp sr) then True else False
+  | {| id, F |} => if RegNameEq.eq rn cwp then True else False
+  | aexp ==ₓ addr => In rn (ApR aexp)
+  | oexp ==ₑ v => In rn (OpR oexp)
+  | _ => False
+  end.
+
+Definition regdisj (p1 : asrt) (p2 : asrt) : Prop :=
+  forall rn, (FR rn p1 -> ~ FR rn p2) /\ (FR rn p2 -> ~ FR rn p1).
 
 (* semantics of assertion language *)
 Fixpoint sat (s : State) (p : asrt) {struct p} : Prop :=
   match p with
-  | Aemp => getmem s = empM /\ getregs s = empR
+  | Aemp => getmem s = empM
   | Amapsto l v => getmem s = MemMap.set l (Some v) empM /\
-                  getregs s = empR /\ word_aligned l = true
+                  word_aligned l = true
   | Aaexpevl aexp addr => eval_addrexp (getregs s) aexp = Some addr /\
-                          word_aligned addr = true
+                      word_aligned addr = true
   | Aoexpevl oexp v => eval_opexp (getregs s) oexp = Some v
   | Areg rn v => regSt rn v s
   | Aregdly t rsp v =>
-    exists v', getregs s = RegMap.set rsp (Some v') empR /\ getmem s = empM /\
-          (regdlySt t rsp v s \/ regSt rsp v s)
-  | Apure p => p /\ getmem s = empM /\ getregs s = empR
+    getmem s = empM /\ (regdlySt t rsp v s \/ regSt rsp v s)
+  | ATimReduce p => exists R D, exe_delay R D = (getregs s, getdlyls s) /\
+                          sat (upddlyls (updregs s R) D) p
+  | Apure p => p /\ getmem s = empM
   | Aframe id F => regSt cwp id s /\ getframelst s = F
+  | Awin p fmo fml fmi => sat (updregs s (replace fmo fml fmi (getregs s))) p
   | Atrue => True
   | Afalse => False
   | Aconj p1 p2 => sat s p1 /\ sat s p2
   | Adisj p1 p2 => sat s p1 \/ sat s p2
   | Astar p1 p2 =>
-    exists s1 s2, state_union s1 s2 s /\ sat s1 p1 /\ sat s2 p2
+    exists s1 s2, state_union s1 s2 s /\ sat s1 p1 /\ sat s2 p2 /\ regdisj p1 p2
   | Aforall t p' => forall (x : t), sat s (p' x)
   | Aexists t p' => exists (x : t), sat s (p' x)
   end.
@@ -196,15 +246,22 @@ Definition InRegs (fm : Frame) : asrt :=
 Definition Regs (fm1 fm2 fm3 : Frame) : asrt :=
   OutRegs fm1 ** LocalRegs fm2 ** InRegs fm3.
 
-Fixpoint DlyFrameFree (a : asrt) :=
+Fixpoint DlyGenRegFree (a : asrt) :=
   match a with
   | t @ rn |==> v => False
-  | {| id, F |} => False
-  | p //\\ q => DlyFrameFree p /\ DlyFrameFree q
-  | p \\// q => DlyFrameFree p /\ DlyFrameFree q
-  | p ** q => DlyFrameFree p /\ DlyFrameFree q
-  | Aforall t p => forall x : t, DlyFrameFree (p x)
-  | Aexists t p => forall x : t, DlyFrameFree (p x)
+  | p //\\ q => DlyGenRegFree p /\ DlyGenRegFree q
+  | p \\// q => DlyGenRegFree p /\ DlyGenRegFree q
+  | p ** q => DlyGenRegFree p /\ DlyGenRegFree q
+  | Aforall t p => forall x : t, DlyGenRegFree (p x)
+  | Aexists t p => forall x : t, DlyGenRegFree (p x)
+  | ATimReduce p => DlyGenRegFree p
+  | Awin p fmo fml fmi => False
+  | rn |=> v => match rn with
+               | Rr rr => False
+               | _ => True
+               end
+  | aexp ==ₓ addr => False
+  | oexp ==ₑ v => False
   | _ => True
   end.
 
@@ -283,18 +340,22 @@ Inductive wf_ins : asrt -> ins -> asrt -> Prop :=
     p ==> {| id, F |} ** rd |=> v' ** p1 ->
     wf_ins p (getcwp rd) ({| id, F |} ** rd |=> id ** p1)
 
-| save_rule : forall p p1 q (rs rd : GenReg) id id' F fm1 fm2 fmo fml fmi v1 v2 v v' oexp,
+| save_rule : forall p p1 q (rs rd : GenReg) id id' F fm1 fm2 v1 v2 v v' oexp,
     p ==> ((Or rs) ==ₑ v1 //\\ oexp ==ₑ v2) ->
-    p ==> {| id, F ++ (fm1 :: fm2 :: nil) |} ** (Regs fmo fml fmi) ** p1 ->
+    p ==> {| id, F ++ (fm1 :: fm2 :: nil) |} ** p1 ->
     id' = pre_cwp id -> win_masked id' v = false ->
-    {| id', fml :: fmi :: F |} ** (Regs fm1 fm2 fmo) ** p1 ==> rd |=> v' ** q ->
+    (forall fmo fml fmi,
+        {| id', fml :: fmi :: F |} ** {[ p1 # fmo, fml, fmi ]} ==>
+                                   {[ rd |=> v' ** q # fm1, fm2, fmo ]}) ->
     wf_ins (Rwim |=> v ** p) (save rs oexp rd) (Rwim |=> v ** rd |=> v1 +ᵢ v2 ** q)
 
-| restore_rule : forall p p1 q (rs rd : GenReg) id id' F fm1 fm2 fmo fml fmi v1 v2 v v' oexp,
+| restore_rule : forall p p1 q (rs rd : GenReg) id id' F fm1 fm2 v1 v2 v v' oexp,
     p ==> ((Or rs) ==ₑ v1 //\\ oexp ==ₑ v2) ->
-    p ==> {| id, fm1 :: fm2 :: F |} ** (Regs fmo fml fmi) ** p1 ->
+    p ==> {| id, fm1 :: fm2 :: F |} ** p1 ->
     id' = post_cwp id -> win_masked id' v = false ->
-    {| id', F ++ (fmo :: fml :: nil)  |} ** (Regs fmi fm1 fm2) ** p1 ==> rd |=> v' ** q ->
+    (forall fmo fml fmi,
+        {| id', F ++ (fmo :: fml :: nil)  |} ** {[ p1 # fmo, fml, fmi ]} ==>
+                                             {[ rd |=> v' ** q # fmi, fm1, fm2 ]}) ->
     wf_ins (Rwim |=> v ** p) (restore rs oexp rd) (Rwim |=> v ** rd |=> v1 +ᵢ v2 ** q)
     
 | ins_conj_rule : forall p1 p2 q1 q2 i,
@@ -310,7 +371,7 @@ Inductive wf_ins : asrt -> ins -> asrt -> Prop :=
     wf_ins p i q
 
 | ins_frame_rule : forall p q r i,
-    wf_ins p i q -> DlyFrameFree r ->
+    wf_ins p i q -> DlyGenRegFree r ->
     wf_ins (p ** r) i (q ** r).
 
 Notation " '|-' '{{' p '}}' i '{{' q '}}' " := (wf_ins p i q) (at level 50).
@@ -333,105 +394,79 @@ Inductive logicvar : Type :=
 Definition fpre := list logicvar -> asrt.
 Definition fpost := list logicvar -> asrt.
 Definition fspec : Type := fpre * fpost.
-Definition funspec := Word * Word -> option fspec.
-
-(* Delay Time Reduce *)
-Fixpoint TimReduce (a : asrt) : asrt :=
-  match a with
-  | p //\\ q => (TimReduce p) //\\ (TimReduce q)
-  | p \\// q => (TimReduce p) \\// (TimReduce q)
-  | p ** q => (TimReduce p) ** (TimReduce q)
-  | Aforall t p => Aforall (fun x : t => (TimReduce (p x)))
-  | Aexists t p => Aexists (fun x : t => (TimReduce (p x)))
-  | Aregdly t rsp v =>
-    match t with
-    | O => rsp |=> v
-    | S t' => t' @ rsp |==> v
-    end
-  | _ => a
-  end.
-Notation "p ↓" := (TimReduce p) (at level 40).
+Definition funspec := Word -> option fspec.
 
 Definition fretSta (p1 p2 : asrt) :=
-  forall s s', s |= p1 -> s' |= p2 ->
-          (exists v, (getregs s) r15 = Some v /\
-                (getregs s') r15 = Some v).
+  forall s s', s |= p1 -> s' |= p2 -> ((getregs s) r15 = (getregs s) r15).
 
-Inductive wf_seq : funspec -> asrt -> InsSeq -> asrt -> Prop :=
+Inductive wf_seq : funspec -> asrt -> Label -> InsSeq -> asrt -> Prop :=
 | seq_rule : forall f i I p p' q Spec,
-    |- {{ p ↓ }} i {{ p' }} -> wf_seq Spec p' I q ->
-    wf_seq Spec p (f # i ;; I) q
+    |- {{ p ↓ }} i {{ p' }} -> wf_seq Spec p' (f +ᵢ ($ 4)) I q ->
+    wf_seq Spec p f (i ;; I) q
 
-| call_rule : forall f f1 f2 i I p p1 p2 p' q r fp fq (L : list logicvar) v (Spec : funspec),
-    Spec (f, f +ᵢ ($ 4)) = Some (fp, fq) ->
+| call_rule : forall f f' i I p p1 p2 p' q r fp fq (L : list logicvar) v (Spec : funspec),
+    Spec f' = Some (fp, fq) ->
     (p ↓) ==> r15 |=> v ** p1 ->
-    |- {{ (r15 |=> f1 ** p1) ↓ }} i {{ p2 }} -> fp L ==> ((Or r15) ==ₑ f1) ->
-    p2 ==> fp L ** r -> fq L ** r ==> p'-> fq L ==> ((Or r15) ==ₑ f1) ->
-    DlyFrameFree r -> wf_seq Spec p' I q ->
-    wf_seq Spec p (f1 c> call f ;; f2 c> i ;; I) q
+    |- {{ (r15 |=> f ** p1) ↓ }} i {{ p2 }} ->
+    p2 ==> fp L ** r -> fq L ** r ==> p'-> fq L ==> ((Or r15) ==ₑ f) ->
+    DlyGenRegFree r -> wf_seq Spec p' (f +ᵢ ($ 8)) I q ->
+    wf_seq Spec p f (call f' # i # I) q
 
-| retl_rule : forall p p' q f1 f2 i Spec,
+| retl_rule : forall p p' q f i Spec,
     |- {{ (p ↓) ↓ }} i {{ p' }} -> p' ==> q -> fretSta ((p ↓) ↓) p' ->
-    wf_seq Spec p (f1 r> retl ;; f2 r> i) q
+    wf_seq Spec p f (retl ;; i) q
 
-| J1_rule : forall p p1 p' q (r1 : GenReg) f f1 f2 aexp Spec fp fq L v r i,
-    (p ↓) ==> aexp ==ₓ f -> Spec (f, f +ᵢ ($ 4)) = Some (fp, fq) ->
-    (p ↓) ==> r1 |=> v ** p1 -> |- {{ (r1 |=> f1 ** p1) ↓ }} i {{ p' }} ->
-    p' ==> fp L ** r -> fq L ** r ==> q -> DlyFrameFree r ->
-    wf_seq Spec p (consJ1 f1 aexp r1 f2 i) q
+| J_rule : forall p p1 p' q (r1 : GenReg) f f' aexp Spec fp fq L v r i,
+    (p ↓) ==> aexp ==ₓ f' -> Spec f' = Some (fp, fq) ->
+    (p ↓) ==> r1 |=> v ** p1 -> |- {{ (r1 |=> f ** p1) ↓ }} i {{ p' }} ->
+    p' ==> fp L ** r -> fq L ** r ==> q -> DlyGenRegFree r ->
+    wf_seq Spec p f (consJ aexp r1 i) q
 
-| J2_rule : forall p p1 p2 q r fp fq L aexp1 aexp2 f1 f1' f2 f2' (r1 r2 : GenReg) v1 v2 Spec,
-    (p ↓) ==> (aexp1 ==ₓ f1') -> (p ↓) ==> r1 |=> v1 ** p1 ->
-    ((r1 |=> f1 ** p1) ↓) ==> (aexp2 ==ₓ f2') -> ((r1 |=> f1 ** p1) ↓) ==> r2 |=> v2 ** p2 ->
-    Spec (f1', f2') = Some (fp, fq) ->
-    (r2 |=> f2 ** p2) ==> fp L ** r -> fq L ** r ==> q -> DlyFrameFree r ->
-    wf_seq Spec p (consJ2 f1 aexp1 r1 f2 aexp2 r2) q
-
-| Be_rule : forall p p' q r f1 f2 f bv fp fq L i I Spec,
-    Spec (f, f +ᵢ ($ 4)) = Some (fp, fq) ->
-    |- {{ p ↓↓ }} i {{ p' }} -> (p ↓) ==> z |=> bv ** Atrue ->
-    (bv =ᵢ ($ 0) = true -> wf_seq Spec p' I q) -> DlyFrameFree r ->
+| Be_rule : forall p p' q bv Spec L f f' r i I fp fq,
+    Spec f' = Some (fp, fq) ->
+    p ==> z |=> bv ** Atrue -> |- {{ p ↓↓ }} i {{ p' }} ->
+    (bv =ᵢ ($ 0) = true -> wf_seq Spec p' (f +ᵢ ($ 8)) I q) -> DlyGenRegFree r ->
     ((bv =ᵢ ($ 0) = false) -> ((p' ==> fp L ** r) /\ (fq L ** r ==> q))) ->
-    wf_seq Spec p (f1 e> be f ;; f2 e> i ;; I) q
+    wf_seq Spec p f (be f' # i # I) q
 
-| Bne_rule : forall p p' q r f1 f2 f bv fp fq L i I Spec,
-    Spec (f, f +ᵢ ($ 4)) = Some (fp, fq) ->
-    |- {{ p ↓↓ }} i {{ p' }} -> (p ↓) ==> z |=> bv ** Atrue ->
-    (bv =ᵢ ($ 0) = false -> wf_seq Spec p' I q) -> DlyFrameFree r ->
+| Bne_rule : forall p p' q bv Spec L f f' r i I fp fq,
+    Spec f' = Some (fp, fq) ->
+    p ==> z |=> bv ** Atrue -> |- {{ p ↓↓ }} i {{ p' }} ->
+    (bv =ᵢ ($ 0) = false -> wf_seq Spec p' (f +ᵢ ($ 8)) I q) -> DlyGenRegFree r ->
     ((bv =ᵢ ($ 0) = true) -> ((p' ==> fp L ** r) /\ (fq L ** r ==> q))) ->
-    wf_seq Spec p (f1 n> bne f ;; f2 n> i ;; I) q
+    wf_seq Spec p f (bne f' # i # I) q
 
-| Seq_false_rule : forall q I Spec,
-    wf_seq Spec Afalse I q
+| Seq_false_rule : forall q I f Spec,
+    wf_seq Spec Afalse f I q
 
-| Seq_frame_rule : forall p q I Spec r,
-    wf_seq Spec p I q -> DlyFrameFree r ->
-    wf_seq Spec (p ** r) I (q ** r )
+| Seq_frame_rule : forall p q I f Spec r,
+    wf_seq Spec p f I q -> DlyGenRegFree r ->
+    wf_seq Spec (p ** r) f I (q ** r )
 
-| Ex_intro_rule : forall q I {tp:Type} p Spec,
-    (forall x', wf_seq Spec (p x') I q) ->
-    wf_seq Spec (EX x : tp, p x) I q
+| Ex_intro_rule : forall q f I {tp:Type} p Spec,
+    (forall x', wf_seq Spec (p x') f I q) ->
+    wf_seq Spec (EX x : tp, p x) f I q
 
-| Seq_conseq_rule : forall p p' q q' I Spec,
-    wf_seq Spec p' I q' -> p ==> p' -> q' ==> q ->
-    wf_seq Spec p I q
+| Seq_conseq_rule : forall p p' q q' f I Spec,
+    wf_seq Spec p' f I q' -> p ==> p' -> q' ==> q ->
+    wf_seq Spec p f I q
 
-| Seq_disj_rule : forall p1 p2 q1 q2 I Spec,
-    wf_seq Spec p1 I q1 -> wf_seq Spec p2 I q2 ->
-    wf_seq Spec (p1 \\// p2) I (q1 \\// q2)
+| Seq_disj_rule : forall p1 p2 q1 q2 f I Spec,
+    wf_seq Spec p1 f I q1 -> wf_seq Spec p2 f I q2 ->
+    wf_seq Spec (p1 \\// p2) f I (q1 \\// q2)
 
-| Pure_intro_rule : forall p q (pu : Prop) I Spec,
-    (pu -> wf_seq Spec p I q) ->
-    wf_seq Spec ([| pu |] ** p) I q.
+| Pure_intro_rule : forall p q (pu : Prop) f I Spec,
+    (pu -> wf_seq Spec p f I q) ->
+    wf_seq Spec ([| pu |] ** p) f I q.
 
-Notation " Spec '|-' '{{' p '}}' I '{{' q '}}' " :=
-  (wf_seq Spec p I q) (at level 55).
+Notation " Spec '|-' '{{' p '}}' f '#' I '{{' q '}}' " :=
+  (wf_seq Spec p f I q) (at level 55).
 
 (*+ Well-formed Code Heap +*)
 Definition wf_cdhp (Spec : funspec) (C : CodeHeap) (Spec' : funspec) :=
-  forall f1 f2 L fp fq,
-    Spec' (f1, f2) = Some (fp, fq) ->
-    exists I, LookupC C f1 f2 I /\ wf_seq Spec (fp L) I (fq L).     
+  forall f L fp fq,
+    Spec' f = Some (fp, fq) ->
+    exists I, LookupC C f I /\ wf_seq Spec (fp L) f I (fq L).
 
 
 
