coqimp/framework/models/language.v
@@ -42,107 +42,81 @@ Inductive command: Type :=
 
 (* Instruction Sequence *)
 Inductive InsSeq : Type :=
-| consSeq : Label -> ins -> InsSeq -> InsSeq
-| consJ1 : Label -> AddrExp -> GenReg ->
-       Label -> ins -> InsSeq
-| consJ2 : Label -> AddrExp -> GenReg ->
-       Label -> AddrExp -> GenReg -> InsSeq
-| consCall : Label -> Label -> Label -> ins -> InsSeq -> InsSeq
-| consRetl : Label -> Label -> ins -> InsSeq
-| consBe : Label -> Label -> Label -> ins -> InsSeq -> InsSeq
-| consBne : Label -> Label -> Label -> ins -> InsSeq -> InsSeq.
+| consSeq : ins -> InsSeq -> InsSeq
+| consJ : AddrExp -> GenReg -> ins -> InsSeq
+| consCall : Label -> ins -> InsSeq -> InsSeq
+| consRetl : ins -> InsSeq
+| consBe : Label -> ins -> InsSeq -> InsSeq
+| consBne : Label -> ins -> InsSeq -> InsSeq.
 
-Notation "f1 # i ;; I" := (consSeq f1 i I) (at level 90, right associativity,
+(* Verified Instruction Sequence *)
+Inductive vInsSeq : Type :=
+| vSeq : Label -> InsSeq -> vInsSeq.
+
+Notation "i ;; I" := (consSeq i I) (at level 90, right associativity,
                                               format
-                                                "f1 # i ;; '//' I"
+                                                "i ;; '//' I"
                                              ): code_scope.
-Notation "f1 > 'jmpl' addr rr ;; f2 > i" := (consJ1 f1 addr rr f2 i)
-                                                  (at level 78, right associativity): code_scope.
-Notation "f1 >> 'Jmpl' addr1 rr1 ;; f2 >> 'Jmpl' addr2 rr2" :=
-  (consJ2 f1 addr1 rr1 f2 addr2 rr2) (at level 78, right associativity): code_scope.
-Notation "f1 c> 'call' f ;; f2 c> i ;; I" :=
-  (consCall f1 f f2 i I) (at level 90, right associativity,
-                                             format
-                                             "f1 c> 'call' f ;; f2 c> i ;; '//' I"
-                         ): code_scope.
-Notation "f1 r> 'retl' ;; f2 r> i" :=
-  (consRetl f1 f2 i) (at level 80, right associativity): code_scope.
-Notation "f1 e> 'be' addr ;; f2 e> i ;; I" :=
-  (consBe f1 addr f2 i I) (at level 90, right associativity,
-                           format
-                             "f1 e> 'be' addr ;; f2 e> i ;; '//' I"
-                          ): code_scope.
-Notation "f1 n> 'bne' addr ;; f2 n> i ;; I" :=
-  (consBne f1 addr f2 i I) (at level 90, right associativity,
-                            format
-                              "f1 n> 'bne' addr ;; f2 n> i ;; '//' I"
-                           ): code_scope.
+Notation "'jmpl' addr rr ;; i" := (consJ addr rr i)
+                                    (at level 78, right associativity): code_scope.
 
-(* Test code *)
-Definition f1 := ($ 1).
-Definition f2 := ($ 2).
-Definition f3 := ($ 3).
-Definition f4 := ($ 4).
+Notation " 'call' f # i # I" :=
+  (consCall f i I) (at level 90, right associativity,
+                    format
+                      "'call' '/' f # i # '//' I"
+                   ): code_scope.
 
-Definition code : InsSeq := 
-  consJ1 f3 (Ao (Or r1)) r3 f4 nop. 
-Print code.
+Notation "'retl' ;; i" :=
+  (consRetl i) (at level 80, right associativity): code_scope.
 
-Definition code1 : InsSeq :=
-  consSeq f1 (add r1 (Or r2) r3) (consJ1 f3 (Ao (Or r1)) r3 f4 nop).
-Print code1.
+Notation "'be' f # i # I" :=
+  (consBe f i I) (at level 90, right associativity,
+                     format
+                       "'be' '/' f # i # '//' I"
+                 ): code_scope.
 
-Definition code2 : InsSeq :=
-  f1 r> retl ;; f2 r> nop.
-
-Definition code3 : InsSeq :=
-  f1 # nop ;; f2 # (add r1 (Or r1) r2) ;;
-                                       f3 r> retl ;; f4 r> nop.
-
-Definition code4 : InsSeq :=
-  f1 c> call f3 ;; f2 c> nop ;; f1 r> retl ;; f2 r> nop.
+Notation "'bne' f # i # I" :=
+  (consBne f i I) (at level 90, right associativity,
+                   format
+                     "'bne' '/' f # i # '//' I"
+                  ): code_scope.
 
 Open Scope code_scope.
 
 (*+ Code Heap +*)
 (* The definition of code heap *)
-Definition CodeHeap := MemMap.t (option command). 
+Definition CodeHeap := MemMap.t (option command).
 
 (* basic code block constructor *)
-Inductive LookupC : CodeHeap -> Label -> Label -> InsSeq -> Prop :=
+Inductive LookupC : CodeHeap -> Label -> InsSeq -> Prop :=
 | lookupNoTransIns :
-    forall C f1 f2 I i,
-      C f1 = Some (cntrans i) -> LookupC C f2 (f2 +ᵢ ($ 4)) I ->
-      LookupC C f1 f2 (f1 # i ;; I)
-| lookupJmp1 :
-    forall C f1 f2 i aexp rr,
-      C f1 = Some (cjumpl aexp rr) ->
-      C f2 = Some (cntrans i) ->
-      LookupC C f1 f2 (consJ1 f1 aexp rr f2 i)
-| lookupJmp2 :
-    forall C f1 f2 aexp1 aexp2 rr1 rr2,
-      C f1 = Some (cjumpl aexp1 rr1) ->
-      C f2 = Some (cjumpl aexp2 rr2) ->
-      LookupC C f1 f2 (consJ2 f1 aexp1 rr1 f2 aexp2 rr2)
+    forall C f I i,
+      C f = Some (cntrans i) -> LookupC C (f +ᵢ ($ 4)) I ->
+      LookupC C f (i ;; I)
+| LookupJmp :
+    forall C f i aexp rr,
+      C f = Some (cjumpl aexp rr) ->
+      C (f +ᵢ ($ 4)) = Some (cntrans i) ->
+      LookupC C f (consJ aexp rr i)
 | lookupRetl :
-    forall C f1 f2 i,
-      C f1 = Some (cretl) -> C f2 = Some (cntrans i) ->
-      LookupC C f1 f2 (f1 r> retl ;; f2 r> i)
+    forall C f i,
+      C f = Some (cretl) -> C (f +ᵢ ($ 4)) = Some (cntrans i) ->
+      LookupC C f (retl ;; i)
 | lookupCall :
-    forall C f1 f2 f i I,
-      C f1 = Some (ccall f) -> C f2 = Some (cntrans i) -> f2 = (f1 +ᵢ ($ 4)) ->
-      LookupC C (f2 +ᵢ ($ 4)) (f2 +ᵢ ($ 8)) I ->
-      LookupC C f1 f2 (f1 c> call f ;; f2 c> i ;; I)
+    forall C f f' i I,
+      C f = Some (ccall f') -> C (f +ᵢ ($ 4)) = Some (cntrans i) ->
+      LookupC C (f +ᵢ ($ 8)) I ->
+      LookupC C f (call f' # i # I)
 | lookupBe :
-    forall C f1 f2 i I f,
-      C f1 = Some (cbe f) -> C f2 = Some (cntrans i) ->
-      LookupC C (f2 +ᵢ ($ 4)) (f2 +ᵢ ($ 8)) I ->
-      LookupC C f1 f2 (f1 e> be f ;; f2 e> i ;; I)
+    forall C f f' i I,
+      C f = Some (cbe f') -> C (f +ᵢ ($ 4)) = Some (cntrans i) ->
+      LookupC C (f +ᵢ ($ 8)) I ->
+      LookupC C f (be f' # i # I)
 | lookupBne :
-    forall C f1 f2 i I f,
-      C f1 = Some (cbne f) -> C f2 = Some (cntrans i) ->
-      LookupC C (f2 +ᵢ ($ 4)) (f2 +ᵢ ($ 8)) I ->
-      LookupC C f1 f2 (f1 n> bne f ;; f2 n> i ;; I).
+    forall C f f' i I,
+      C f = Some (cbne f') -> C (f +ᵢ ($ 4)) = Some (cntrans i) ->
+      LookupC C (f +ᵢ ($ 8)) I ->
+      LookupC C f (bne f' # i # I).
 
 (*+ Operational Semantics +*)
 
@@ -155,10 +129,10 @@ Definition word_aligned: Word -> bool :=
 Definition iszero v :=
   if Int.eq_dec v ($ 0) then $ 1 else $ 0.
 
-Fixpoint set_Rs R (vl : list (RegName * Word)) :=
-  match vl with
-  | (rr, w) :: vl =>
-    set_Rs (set_R R rr w) vl
+Fixpoint set_Rs (R : RegFile) (lv : list (RegName * Word)) :=
+  match lv with
+  | (rn, v) :: lv' =>
+    set_Rs (RegMap.set rn v R) lv'
   | nil => R
   end.
 
@@ -166,85 +140,68 @@ Fixpoint set_Rs R (vl : list (RegName * Word)) :=
 Inductive R__ : Memory * RegFile -> ins -> Memory * RegFile -> Prop :=
 | Ld_step : forall aexp (ri : GenReg) M R R' addr v,
     eval_addrexp R aexp = Some addr -> word_aligned addr = true ->
-    M addr = Some v -> indom ri R -> set_R R ri v = R' ->
+    M addr = Some v -> RegMap.set ri v R = R' ->
     R__ (M, R) (ld aexp ri) (M, R')
 
 | ST_step : forall (ri : GenReg) aexp M M' R addr v,
     eval_addrexp R aexp = Some addr -> word_aligned addr = true ->
-    get_R R ri = Some v -> indom addr M -> MemMap.set addr (Some v) M = M' ->
+    get_R R ri = v -> indom addr M -> MemMap.set addr (Some v) M = M' ->
     R__ (M, R) (st ri aexp) (M', R)
 
 | Nop_step : forall M R,
     R__ (M, R) nop (M, R)
 
 | Add_step : forall M (R R' : RegFile) oexp (rs rd : GenReg) v1 v2,
-    get_R R rs = Some v1 -> eval_opexp R oexp = Some v2 ->
-    indom rd R -> set_R R rd (v1 +ᵢ v2) = R' ->
+    get_R R rs = v1 -> eval_opexp R oexp = Some v2 ->
+    RegMap.set rd (v1 +ᵢ v2) R = R' ->
     R__ (M, R) (add rs oexp rd) (M, R')
         
 | Sub_step : forall M (R R' : RegFile) oexp (rs rd : GenReg) v1 v2,
-    get_R R rs = Some v1 -> eval_opexp R oexp = Some v2 ->
-    indom rd R -> set_R R rd (v1 -ᵢ v2) = R' ->
+    get_R R rs = v1 -> eval_opexp R oexp = Some v2 ->
+    RegMap.set rd (v1 -ᵢ v2) R = R' ->
     R__ (M, R) (sub rs oexp rd) (M, R')
 
 | Subcc_step : forall M (R R' : RegFile) oexp (rs rd : GenReg) v1 v2 v,
-    get_R R rs = Some v1 -> eval_opexp R oexp = Some v2 ->
-    indom rd R -> indom n R -> indom z R -> v = v1 -ᵢ v2 ->
+    get_R R rs = v1 -> eval_opexp R oexp = Some v2 -> v = v1 -ᵢ v2 ->
     set_Rs R ((Rr rd, v) :: (Rpsr n, get_range 31 31 v) :: (Rpsr z, iszero v) :: nil) = R' ->
     R__ (M, R) (subcc rs oexp rd) (M, R')
 
 | And_step : forall M (R R' : RegFile) oexp (rs rd : GenReg) v1 v2,
-    get_R R rs = Some v1 -> eval_opexp R oexp = Some v2 ->
-    indom rd R -> set_R R rd (v1 &ᵢ v2) = R' ->
+    get_R R rs = v1 -> eval_opexp R oexp = Some v2 ->
+    RegMap.set rd (v1 &ᵢ v2) R = R' ->
     R__ (M, R) (and rs oexp rd) (M, R')
 
 | Andcc_step : forall M (R R' : RegFile) oexp (rs rd : GenReg) v1 v2 v,
-    get_R R rs = Some v1 -> eval_opexp R oexp = Some v2 ->
-    indom rd R -> indom n R -> indom z R -> v = v1 &ᵢ v2 ->
+    get_R R rs = v1 -> eval_opexp R oexp = Some v2 -> v = v1 &ᵢ v2 ->
     set_Rs R ((Rr rd, v) :: (Rpsr n, get_range 31 31 v) :: (Rpsr z, iszero v) :: nil) = R' ->
     R__ (M, R) (andcc rs oexp rd) (M, R')
 
 | Or_step : forall M (R R' : RegFile) oexp (rs rd : GenReg) v1 v2,
-    get_R R rs = Some v1 -> eval_opexp R oexp = Some v2 ->
-    indom rd R -> set_R R rd (v1 |ᵢ v2) = R' ->
+    get_R R rs = v1 -> eval_opexp R oexp = Some v2 ->
+    RegMap.set rd (v1 |ᵢ v2) R = R' ->
     R__ (M, R) (or rs oexp rd) (M, R')
 
 | Sll_step : forall M (R R' : RegFile) oexp (rs rd : GenReg) v1 v2,
-    get_R R rs = Some v1 -> eval_opexp R oexp = Some v2 ->
-    indom rd R -> set_R R rd (v1 <<ᵢ (get_range 0 4 v2)) = R' ->
+    get_R R rs = v1 -> eval_opexp R oexp = Some v2 ->
+    RegMap.set rd (v1 <<ᵢ (get_range 0 4 v2)) R = R' ->
     R__ (M, R) (sll rs oexp rd) (M, R')
 
 | Srl_step : forall M (R R' : RegFile) oexp (rs rd : GenReg) v1 v2,
-    get_R R rs = Some v1 -> eval_opexp R oexp = Some v2 ->
-    indom rd R -> set_R R rd (v1 >>ᵢ (get_range 0 4 v2)) = R' ->
+    get_R R rs = v1 -> eval_opexp R oexp = Some v2 ->
+    RegMap.set rd (v1 >>ᵢ (get_range 0 4 v2)) R = R' ->
     R__ (M, R) (srl rs oexp rd) (M, R')
 
 | Set_step : forall M (R R' : RegFile) (rd : GenReg) w,
-    indom rd R -> set_R R rd w = R' ->
+    RegMap.set rd w R = R' ->
     R__ (M, R) (sett w rd) (M, R')
 
 | Rd_step : forall M (R R' : RegFile) (rsp : SpReg) (ri : GenReg) v,
-    get_R R rsp = Some v -> indom ri R -> set_R R ri v = R' ->
+    get_R R rsp = v -> RegMap.set ri v R = R' ->
     R__ (M, R) (rd rsp ri) (M, R')
 
 | GetCwp_step : forall M (R R' : RegFile) (ri : GenReg) v,
-    get_R R cwp = Some v -> indom ri R -> set_R R ri v = R' ->
+    get_R R cwp = v -> RegMap.set ri v R = R' ->
     R__ (M, R) (getcwp ri) (M, R').
-
-(* Operation to write a frame *)
-Definition set_frame R (rr0 rr1 rr2 rr3 rr4 rr5 rr6 rr7 : GenReg) (fm : Frame) :=
-  match fm with
-  | consfm w0 w1 w2 w3 w4 w5 w6 w7 =>
-    set_Rs R
-           ((Rr rr0, w0) :: (Rr rr1, w1) :: (Rr rr2, w2) :: (Rr rr3, w3) :: (Rr rr4, w4) ::
-                         (Rr rr5, w5) :: (Rr rr6, w6) :: (Rr rr7, w7) :: nil)
-  end.
-
-(* Operation to write a window *)
-Definition set_window R (fm1 fm2 fm3 : Frame) :=
-  let R1 := set_frame R r8 r9 r10 r11 r12 r13 r14 r15 fm1 in
-  let R2 := set_frame R1 r16 r17 r18 r19 r20 r21 r22 r23 fm2 in
-  set_frame R2 r24 r25 r26 r27 r28 r29 r30 r31 fm3.
 
 Definition N := $ 8.
 
@@ -272,28 +229,28 @@ Inductive Q__: State -> command -> State -> Prop :=
 
 | SSave :
     forall (M : Memory) (R R' R'': RegFile) D F F' k k' oexp
-           fmo fml fmi fm1 fm2 v1 v2 v (rs rd : GenReg),
-      get_R R cwp = Some k -> get_R R Rwim = Some v ->
-      fetch R = Some [fmo; fml; fmi] -> indom rd R -> 
-      get_R R rs = Some v1 -> eval_opexp R oexp = Some v2 -> F = F' ++ (fm1 :: fm2 :: nil) ->
-      R' = set_window R fm1 fm2 fmo -> k' = pre_cwp k -> win_masked k' v = false -> 
+      fmo fml fmi fm1 fm2 v1 v2 v (rs rd : GenReg),
+      get_R R cwp = k -> get_R R Rwim = v ->
+      fetch R = (fmo, fml, fmi) ->
+      get_R R rs = v1 -> eval_opexp R oexp = Some v2 -> F = F' ++ (fm1 :: fm2 :: nil) ->
+      R' = replace fm1 fm2 fmo R -> k' = pre_cwp k -> win_masked k' v = false ->
       R'' = set_Rs R' ((Rpsr cwp, k') :: (Rr rd, v1 +ᵢ v2) :: nil) ->
       Q__ (M, (R, F), D) (cntrans (save rs oexp rd)) (M, (R'', fml :: fmi :: F'), D)
 
 | RRestore :
     forall (M : Memory) (R R' R'': RegFile) D F F' k k' oexp
-           fmo fml fmi fm1 fm2 v1 v2 v (rs rd : GenReg),
-      get_R R cwp = Some k -> get_R R Rwim = Some v ->
-      fetch R = Some [fmo; fml; fmi] -> indom rd R ->
-      get_R R rs = Some v1 -> eval_opexp R oexp = Some v2 -> F = fm1 :: fm2 :: F' ->
-      R' = set_window R fmi fm1 fm2 -> k' = post_cwp k -> win_masked k' v = false ->
+      fmo fml fmi fm1 fm2 v1 v2 v (rs rd : GenReg),
+      get_R R cwp = k -> get_R R Rwim = v ->
+      fetch R = (fmo, fml, fmi) ->
+      get_R R rs = v1 -> eval_opexp R oexp = Some v2 -> F = fm1 :: fm2 :: F' ->
+      R' = replace fmi fm1 fm2 R -> k' = post_cwp k -> win_masked k' v = false ->
       R'' = set_Rs R' ((Rpsr cwp, post_cwp k) :: (Rr rd, v1 +ᵢ v2) :: nil) ->
       Q__ (M, (R, F), D) (cntrans (restore rs oexp rd)) (M, (R'', F' ++ (fmo :: fml :: nil)), D)
-
+      
 | Wr :
     forall M (R : RegFile) F D D' (rs : GenReg) (rsp : SpReg) oexp v1 v2 v,
-      get_R R rs = Some v1 -> eval_opexp R oexp = Some v2 ->
-      v = set_spec_reg rsp (v1 xor v2) -> indom rsp R -> D' = set_delay rsp v D ->
+      get_R R rs = v1 -> eval_opexp R oexp = Some v2 ->
+      v = set_spec_reg rsp (v1 xor v2) -> D' = set_delay rsp v D ->
       Q__ (M, (R, F), D) (cntrans (wr rs oexp rsp)) (M, (R, F), D').
 
 (* Operation Semantics for Control Transfer *)
@@ -306,37 +263,37 @@ Inductive H__ : CodeHeap -> State * Label * Label -> State * Label * Label -> Pr
 | Jumpl :
     forall C M aexp rd (R R' : RegFile) F D (pc npc f : Label),
       C pc = Some (cjumpl aexp rd) -> eval_addrexp R aexp = Some f ->
-      word_aligned f = true -> indom rd R -> set_R R rd pc = R' ->
+      word_aligned f = true -> RegMap.set rd pc R = R' ->
       H__ C ((M, (R, F), D), pc, npc) ((M, (R', F), D), npc, f)
 
 | Call :
     forall C M (R R' : RegFile) F D pc npc f,
-      C pc = Some (ccall f) -> indom r15 R -> set_R R r15 pc = R' ->
+      C pc = Some (ccall f) -> RegMap.set r15 pc R = R' ->
       H__ C ((M, (R, F), D), pc, npc) ((M, (R', F), D), npc, f)
 
 | Retl :
     forall C M (R : RegFile) F D pc npc f,
-      C pc = Some (cretl) -> get_R R r15 = Some f ->
+      C pc = Some (cretl) -> get_R R r15 = f ->
       H__ C ((M, (R, F), D), pc, npc) ((M, (R, F), D), npc, f +ᵢ ($ 8))
 
 | Be_true :
     forall C M (R : RegFile) F D pc npc f v,
-      C pc = Some (cbe f) -> get_R R z = Some v -> v <> ($ 0) ->
+      C pc = Some (cbe f) -> get_R R z = v -> v <> ($ 0) ->
       H__ C ((M, (R, F), D), pc, npc) ((M, (R, F), D), npc, f)
 
 | Be_false :
     forall C M (R : RegFile) F D pc npc f,
-      C pc = Some (cbe f) -> get_R R z = Some ($ 0) ->
+      C pc = Some (cbe f) -> get_R R z = ($ 0) ->
       H__ C ((M, (R, F), D), pc, npc) ((M, (R, F), D), npc, npc +ᵢ ($ 4))
 
 | Bne_true :
     forall C M (R : RegFile) F D pc npc f,
-      C pc = Some (cbne f) -> get_R R z = Some ($ 0) ->
+      C pc = Some (cbne f) -> get_R R z = ($ 0) ->
       H__ C ((M, (R, F), D), pc, npc) ((M, (R, F), D), npc, f)
 
 | Bne_false :
     forall C M (R : RegFile) F D pc npc f v,
-      C pc = Some (cbne f) -> get_R R z = Some v -> v <> ($ 0) ->
+      C pc = Some (cbne f) -> get_R R z = v -> v <> ($ 0) ->
       H__ C ((M, (R, F), D), pc, npc) ((M, (R, F), D), npc, npc +ᵢ ($ 4)).
 
 Inductive P__ : CodeHeap -> State * Label * Label -> State * Label * Label -> Prop :=
