coqimp/example/lib/sep_lemma.v
@@ -1,0 +1,948 @@
+Require Import Coqlib.        
+Require Import Maps.      
+Require Import LibTactics.  
+        
+Require Import Integers.  
+Open Scope Z_scope.    
+Import ListNotations.
+  
+Set Asymmetric Patterns.  
+       
+Require Import state.    
+Require Import language. 
+
+Set Implicit Arguments.  
+Unset Strict Implicit. 
+              
+Require Import logic.
+   
+Require Import lemmas.
+(*Require Import lemmas_ins.*)
+
+Require Import Coq.Logic.FunctionalExtensionality.
+  
+Open Scope nat.
+Open Scope code_scope.
+Open Scope mem_scope.
+
+Definition FReq (p1 p2 : asrt) :=
+  forall rn, (FR rn p1 -> FR rn p2) /\ (FR rn p2 -> FR rn p1).
+
+Lemma astar_subst1 :
+  forall p1 p1' p2 s,
+    s |= p1 ** p2 -> p1 ==> p1' ->
+    FReq p1 p1' ->
+    s |= p1' ** p2.
+Proof. 
+  intros.
+  sep_star_split_tac.
+  simpl in H5.
+  simpl.
+  simpljoin1. 
+  exists (m, (r0, f0), d0) (m0, (r0, f0), d0).
+  simpl.
+  do 3 (split; eauto).
+  unfolds regdisj.
+  intros.
+  specialize (H6 rn).
+  simpljoin1.
+  unfolds FReq.
+  specialize (H1 rn).
+  simpljoin1.
+  split.
+  intro.
+  eauto.
+  intro.
+  intro.
+  eapply H6 in H8.
+  eapply H3 in H8.
+  tryfalse.
+Qed.
+
+Lemma astar_subst2 :
+  forall p1 p2 p2' s,
+    s |= p1 ** p2 -> p2 ==> p2' ->
+    FReq p2 p2' ->
+    s |= p1 ** p2'.
+Proof.
+  intros.
+  sep_star_split_tac.
+  simpl in H5.
+  simpl.
+  simpljoin1.
+  exists (m, (r0, f0), d0) (m0, (r0, f0), d0).
+  simpl.
+  split; eauto.
+  do 2 (split; eauto).
+  clear - H6 H1.
+  unfolds regdisj.
+  intro.
+  specialize (H6 rn).
+  simpljoin1.
+  unfolds FReq.
+  specialize (H1 rn).
+  simpljoin1.
+  split; intro; eauto.
+  intro.
+  eapply H2 in H4.
+  eapply H0 in H4.
+  tryfalse.
+Qed.
+
+Theorem astar_assoc_intro :
+  forall P Q R, P ** Q ** R ==> (P ** Q) ** R.
+Proof.
+  intros.
+  eapply sep_star_assoc; eauto.
+Qed.
+
+Theorem astar_assoc_elim :
+  forall P Q R, (P ** Q) ** R ==> P ** Q ** R.
+Proof.
+  intros.
+  eapply sep_star_assoc2; eauto.
+Qed.
+
+Theorem astar_comm :
+  forall P Q,
+    P ** Q ==> Q ** P.
+Proof.
+  intros.
+  eapply sep_star_sym; eauto.
+Qed.
+
+Lemma merge_empM_r_eq :
+  forall M,
+    merge M empM = M.
+Proof.
+  intros.
+  unfold merge.
+  eapply functional_extensionality; eauto.
+  intro.
+  destruct (M x); eauto.
+Qed.
+
+Lemma merge_empM_l_eq :
+  forall M,
+    merge empM M = M.
+Proof.
+  intros.
+  unfold merge.
+  eapply functional_extensionality; eauto.
+Qed.
+  
+Lemma astar_emp_intro_r :
+  forall p,
+    p ==> p ** Aemp.
+Proof.
+  intros.
+  destruct_state s.
+  simpl.
+  exists (m, (r, f), d) (empM, (r, f), d).
+  simpl.
+  repeat (split; eauto).
+  unfold disjoint.
+  intro.
+  destruct (m x); simpl; eauto.
+  rewrite merge_empM_r_eq; eauto.
+Qed.
+
+Lemma astar_emp_elim_r :
+  forall p,
+    p ** Aemp ==> p.
+Proof.
+  intros.
+  sep_star_split_tac.
+  simpl in H3.
+  simpljoin1.
+  simpl in H2.
+  simpljoin1.
+  rewrite merge_empM_r_eq; eauto.
+Qed.
+  
+Lemma astar_emp_intro_l :
+  forall p, 
+    p ==> Aemp ** p.
+Proof.
+  intros.
+  destruct_state s.
+  simpl.
+  exists (empM, (r, f), d) (m, (r, f), d).
+  simpls.
+  repeat (split; eauto).
+  unfold disjoint.
+  intro.
+  simpl; eauto.
+  destruct (m x); eauto.
+Qed.
+
+Lemma astar_emp_elim_l :
+  forall p,
+    Aemp ** p ==> p.
+Proof.
+  intros.
+  sep_star_split_tac.
+  simpls.
+  simpljoin1.
+  eauto.
+Qed.
+  
+Ltac sassocr_in H :=
+  match type of H with
+    | _ |= (_ ** _) ** _ => apply astar_assoc_elim in H; sassocr_in H
+    | _ => idtac
+  end.
+
+Ltac sassocl_in H :=
+  match type of H with
+    | _ |= _ ** (_ ** _) => apply astar_assoc_intro in H; sassocr_in H
+    | _ => idtac
+  end.
+
+Ltac sassocr :=
+  match goal with
+    | |- _ |= (_ ** _) ** _ => apply astar_assoc_intro; sassocr
+    | _ => idtac
+  end.
+
+Ltac sassocl :=
+  match goal with
+    | |- _ |= _ ** (_ ** _) => apply astar_assoc_elim; sassocl
+    | _ => idtac
+  end.
+
+Ltac scomm_in H :=
+  match type of H with
+    | _ |= _ ** _ => apply astar_comm in H
+    | _ => idtac
+  end.
+
+Ltac scomm :=
+  match goal with
+    | |- _ |= _ ** _ => apply astar_comm
+    | _ => idtac
+  end.
+
+Tactic Notation "sep" "assocr" "in" hyp (H) :=
+  sassocr_in H.
+Tactic Notation "sep" "assocl" "in" hyp (H) :=
+  sassocl_in H.
+Tactic Notation "sep" "assocr" :=
+  sassocr.
+Tactic Notation "sep" "assocl" :=
+  sassocl.
+Tactic Notation "sep" "comm" "in" hyp (H) :=
+  scomm_in H.
+Tactic Notation "sep" "comm" :=
+  scomm.
+
+Ltac sliftn n :=
+  match eval compute in n with
+    | 0%nat => idtac
+    | 1%nat => sep assocr
+    | S ?n' => sep assocr; sep comm; sliftn n'
+  end.
+
+Ltac sliftn_in H n :=
+  match eval compute in n with
+    | 0%nat => idtac
+    | 1%nat => sep assocr in H
+    | S ?n' => sep assocr in H; sep comm in H; sliftn_in H n'
+  end.
+
+Fixpoint asrt_get_nth n p :=
+  match n with
+  | O => match p with
+        | p1 ** p2 => p1
+        | _ => p
+        end
+  | S n' =>
+    match p with
+    | p1 ** p2 => asrt_get_nth n' p2
+    | _ => Aemp
+    end
+  end.
+
+Fixpoint asrt_rm_nth n p :=
+  match n with
+  | O => match p with
+        | p1 ** p2 => p2
+        | _ => Aemp
+        end
+  | S n' =>
+    match p with
+    | p1 ** p2 => p1 ** asrt_rm_nth n' p2
+    | _ => p
+    end
+  end.
+
+Lemma FR_get_rm_stable_rev :
+  forall p rn n,
+    FR rn (asrt_get_nth n p) \/ FR rn (asrt_rm_nth n p) ->
+    FR rn p.
+Proof.
+  intro p.
+  induction p; intros;
+    try solve [simpls; eauto; tryfalse];
+    try solve [destruct n; simpls; eauto; try destruct H; tryfalse; eauto].
+
+  {
+    destruct n0.
+    simpl in H.
+    destruct_rneq_H.
+    subst; eauto.
+    simpl; eauto.
+    destruct_rneq.
+    destruct H; tryfalse.
+    simpl in H.
+    destruct_rneq_H.
+    subst.
+    simpl; eauto.
+    destruct_rneq.
+    destruct H; tryfalse.
+  }
+
+  {
+    destruct n.
+    simpl in H.
+    simpl; eauto.
+    simpl in H.
+    assert (FR rn p1 \/ FR rn (asrt_get_nth n p2) \/ FR rn (asrt_rm_nth n p2)).
+    {
+      destruct H; eauto.
+      destruct H; eauto.
+    }
+    destruct H0.
+    simpl; eauto.
+    eapply IHp2 in H0.
+    simpl; eauto.
+  }
+
+  destruct n.
+  simpl in H0.
+  destruct H0; tryfalse.
+  simpl; eauto.
+  simpl in H0.
+  destruct H0; tryfalse.
+  simpl; eauto.
+
+  destruct n.
+  simpl in H0.
+  destruct H0; tryfalse.
+  simpl; eauto.
+  simpl in H0.
+  destruct H0; tryfalse.
+  simpl; eauto.
+Qed.
+
+Lemma FR_get_rm_stable :
+  forall p rn n,
+    FR rn p ->
+    FR rn (asrt_get_nth n p) \/ FR rn (asrt_rm_nth n p).
+Proof.
+  intro p.
+  induction p; intros;
+    try solve [simpls; eauto; tryfalse];
+    try solve [destruct n; simpls; eauto].
+
+  {
+    simpl in H.
+    destruct_rneq_H; tryfalse.
+    subst.
+    destruct n0; simpl; eauto.
+    destruct_rneq.
+    destruct_rneq.
+  }
+
+  simpl in H.
+  destruct H.
+  {
+    eapply IHp1 with (n := n) in H.
+    destruct n.
+    simpl. 
+    left.
+    simpl.
+    eapply FR_get_rm_stable_rev; eauto.
+    right.
+    left.
+    eapply FR_get_rm_stable_rev; eauto.
+  }
+  {
+    eapply IHp2 with (n := n) in H.
+    destruct n.
+    simpl.
+    right.
+    eapply FR_get_rm_stable_rev; eauto.
+    simpl.
+    eapply FR_get_rm_stable_rev in H.
+    eapply or_assoc.
+    assert (FR rn (asrt_get_nth n p2) \/ FR rn p1 <-> FR rn p1 \/ FR rn (asrt_get_nth n p2)).
+    {
+      eapply or_comm; eauto.
+    }
+    rewrite H0.
+    eapply or_assoc.
+    right.
+    eapply IHp2; eauto.
+  }
+Qed.
+  
+Lemma FReq_get_rm_stable :
+  forall p n,
+    FReq p (asrt_get_nth n p ** asrt_rm_nth n p).
+Proof.
+  intros.
+  unfolds FReq.
+  intro.
+  split.
+  {
+    simpl.
+    intro.
+    eapply FR_get_rm_stable; eauto.
+  }
+  {
+    intro.
+    simpl in H.
+    eapply FR_get_rm_stable_rev in H; eauto.
+  }
+Qed.
+
+Lemma FReq_sym :
+  forall p1 p2,
+    FReq p1 p2 <-> FReq p2 p1.
+Proof.
+  intros.
+  split.
+  intro.
+  unfolds FReq.
+  intro.
+  specialize (H rn).
+  simpljoin1; eauto.
+  unfolds FReq.
+  intro.
+  intro.
+  specialize (H rn).
+  simpljoin1; eauto.
+Qed.
+  
+Lemma asrt_lift_nth_stable :
+  forall n p s,
+    s |= p ->
+    s |= asrt_get_nth n p ** asrt_rm_nth n p.
+Proof. 
+  intro n.
+  induction n; intros.
+  -
+    destruct p;
+      simpl asrt_get_nth; simpl asrt_rm_nth;
+        try solve [eapply astar_emp_intro_r; eauto].
+    eauto.
+  -
+    destruct p;
+      simpl asrt_get_nth; simpl asrt_rm_nth;
+        try solve [eapply astar_emp_intro_l; eauto].
+    specialize (IHn p2).
+    eapply astar_subst2 in H; eauto.
+    eapply sep_star_lift in H; eauto. 
+    eapply FReq_get_rm_stable; eauto.
+Qed.
+
+Lemma asrt_lift_nth_stable_rev :
+  forall n p s,
+    s |= asrt_get_nth n p ** asrt_rm_nth n p ->
+    s |= p.
+Proof.
+  intro n.
+  induction n; intros.
+  -
+    destruct p;
+      try solve
+          [
+            simpls asrt_get_nth; simpls asrt_rm_nth;
+            eapply astar_emp_elim_r in H; eauto
+          ].
+    simpls; eauto.
+  -
+    destruct p;
+      try solve
+          [
+            simpls asrt_get_nth; simpls asrt_rm_nth;
+            eapply astar_emp_elim_l in H; eauto
+          ].
+    simpl asrt_get_nth in H.
+    simpl asrt_rm_nth in H.
+    specialize (IHn p2).
+    eapply sep_star_lift in H.
+    eapply astar_subst2 in H; eauto.
+    eapply FReq_sym; eauto.
+    eapply FReq_get_rm_stable.
+Qed.
+
+Ltac simpl_sep_liftn_in H t :=
+  match t with
+  | 0%nat => idtac "n stars from 1, not 0"
+  | S ?n' =>
+    match type of H with
+    | _ |= _ =>
+        eapply asrt_lift_nth_stable with (n := n') in H;
+        unfold asrt_get_nth in H; unfold asrt_rm_nth in H;
+        try eapply astar_emp_elim_l in H;
+        try eapply astar_emp_elim_r in H
+    | _ => idtac "no assertion"
+    end
+  end.
+
+Ltac simpl_sep_liftn t :=
+  match t with
+  | 0%nat => idtac "n stars from 1, not 0"
+  | S ?n' =>
+    match goal with
+    | |- _ |= _ =>
+      eapply asrt_lift_nth_stable_rev with (n := n');
+      unfold asrt_get_nth; unfold asrt_rm_nth;
+      try eapply astar_emp_intro_r;
+      try eapply astar_emp_intro_l
+    | _ => idtac "no assertion"
+    end
+  end.
+
+Fixpoint asrt_combine_to_line (p1 : asrt) (p2 : asrt) (n : nat) :=
+  match p1 with
+  | p1' ** p2' => match n with
+                 | 0%nat => p1 ** p2
+                 | S n' => p1' ** (asrt_combine_to_line p2' p2 n')
+                 end
+  | _ => p1 ** p2
+  end.
+
+Lemma FR_combine_to_line_stable :
+  forall p1 p2 rn n,
+    FR rn (asrt_combine_to_line p1 p2 n) ->
+    FR rn (p1 ** p2).
+Proof.
+  intro p1.
+  induction p1; intros; simpl;
+    try solve [destruct n; simpl in H; try destruct H; tryfalse; eauto].
+
+  destruct n.
+  {
+    simpl in H.
+    eauto.
+  }
+  {
+    simpl in H.
+    destruct H; eauto.
+    eapply IHp1_2 in H.
+    simpl in H.
+    destruct H; eauto.
+  }
+Qed.
+
+Lemma FR_combine_to_line_stable_rev :
+  forall p1 p2 rn n,
+    FR rn (p1 ** p2) ->
+    FR rn (asrt_combine_to_line p1 p2 n).
+Proof.
+  intro p1.
+  induction p1; intros; simpl;
+    try solve [simpls; destruct H; tryfalse; eauto].
+
+  {
+    destruct n.
+    eauto.
+    simpl in H.
+    rewrite or_assoc in H.
+    destruct H; simpl; eauto.
+  }
+
+  simpl; eauto.
+  simpl; eauto.
+Qed.
+  
+Lemma regdisj_combine_to_line_stable :
+  forall p1 p2 p3 n,
+    regdisj p1 (p2 ** p3) ->
+    regdisj p1 (asrt_combine_to_line p2 p3 n).
+Proof.
+  intros.
+  unfolds regdisj.
+  intro.
+  specialize (H rn).
+  simpljoin1.
+  split.
+  {
+    intro.
+    eapply H in H1.
+    intro.
+    eapply H1.
+    eapply FR_combine_to_line_stable; eauto.
+  }
+  {
+    intro.
+    intro.
+    eapply FR_combine_to_line_stable in H1.
+    eapply H0 in H1.
+    tryfalse.
+  }
+Qed.
+  
+Lemma asrt_combine_to_line_stable :
+  forall n p1 p2 s,
+    s |= p1 ** p2 ->
+    s |= asrt_combine_to_line p1 p2 n.
+Proof.
+  intro n.
+  induction n; intros.
+  -
+    destruct p1; simpls; eauto.
+  - 
+    destruct p1;
+      try solve [simpls; eauto].
+    simpl.
+    sep_star_split_tac.
+    simpl in H1, H3.
+    simpljoin1.
+    exists (m1, (r2, f2), d2) (merge m2 m0, (r2, f2), d2).
+    split; eauto.
+    repeat (split; eauto).
+    eapply disj_sep_merge_still; eauto.
+    eapply disj_sym in H3.
+    eapply disj_merge_disj_sep1 in H3; eauto.
+    eapply disj_sym; eauto.
+    rewrite merge_assoc; eauto.
+    split; eauto.
+    split.
+    eapply IHn; eauto. 
+    simpl.
+    do 2 eexists.
+    split; eauto.
+    Focus 2. 
+    split; eauto.
+    split; eauto.
+    eapply regdisj_star_sepl2 in H4.
+    eauto.
+    simpl. 
+    repeat (split; eauto).
+    eapply disj_sym in H3.
+    eapply disj_merge_disj_sep2 in H3.
+    eapply disj_sym; eauto.
+    eapply regdisj_star_sepl1 in H4.
+    assert (regdisj p1_1 (p1_2 ** p2)).
+    eapply regdisj_star_merge; eauto.
+    eapply regdisj_combine_to_line_stable; eauto.
+Qed.
+
+Lemma FReq_combine_to_line_stable :
+  forall p1 p2 n,
+    FReq (p1 ** p2) (asrt_combine_to_line p1 p2 n).
+Proof.
+  intros.
+  unfolds FReq.
+  intros.
+  split; eauto.
+  intro.
+  eapply FR_combine_to_line_stable_rev; eauto.
+  intro.
+  eapply FR_combine_to_line_stable; eauto.
+Qed.
+
+Lemma asrt_combine_to_line_stable_rev :
+  forall n p1 p2 s,
+    s |= asrt_combine_to_line p1 p2 n ->
+    s |= p1 ** p2.
+Proof.
+  intro n.
+  induction n; intros.
+  -
+    destruct p1; simpls; eauto.
+  -
+    destruct p1;
+      try solve [simpls; eauto].
+    simpl asrt_combine_to_line in H.
+    eapply astar_assoc_intro; eauto.
+    eapply astar_subst2; eauto.
+    eapply FReq_sym; eauto.
+    eapply FReq_combine_to_line_stable; eauto.
+Qed.
+
+Inductive asrtTree : Type :=
+| empTree : asrtTree
+| trueTree : asrtTree
+| starTree : asrtTree -> asrtTree -> asrtTree
+| pureTree : Prop -> asrtTree
+| baseTree : asrt -> asrtTree.
+
+Fixpoint toTree Hp :=
+  match Hp with
+    | A ** B => let tA := toTree A in
+                  let tB := toTree B in
+                  starTree tA tB
+    | Aemp => empTree
+    | Atrue => trueTree
+    | [| P |] => pureTree P
+    | _ => baseTree Hp
+  end.
+
+Fixpoint unTree (t:asrtTree) : asrt :=
+  match t with
+    | empTree => Aemp
+    | trueTree => Atrue
+    | starTree A B => unTree A ** unTree B
+    | pureTree P => [| P |]
+    | baseTree A => A
+  end.
+
+Fixpoint asrtTree_to_list' (Hp:asrtTree) (l:list asrtTree) : list asrtTree :=
+  match Hp with
+    | starTree A B => asrtTree_to_list' A (asrtTree_to_list' B l)
+    | _ => Hp::l
+  end.
+
+Definition asrtTree_to_list (Hp:asrtTree) : list asrtTree :=
+  asrtTree_to_list' Hp nil.
+
+Fixpoint asrt_to_list' Hp l :=
+  match Hp with
+    | A ** B => let rl := asrt_to_list' B l in
+                  asrt_to_list' A rl
+    | A => A :: l
+  end.
+Definition asrt_to_list Hp := asrt_to_list' Hp (@nil asrt).
+
+Fixpoint list_to_asrt l :=
+  match l with
+  | nil => Aemp
+  | A :: l' => let ar := list_to_asrt l' in
+              A ** ar
+  end.
+
+Lemma asrt_to_list'_assoc :
+  forall p1 p2 p3 l,
+    asrt_to_list' ((p1 ** p2) ** p3) l =
+    asrt_to_list' (p1 ** p2 ** p3) l.
+Proof.
+  intro p1.
+  induction p1; intros;
+    try solve [simpl; eauto].
+Qed.
+
+Lemma asrt_to_list_app :
+  forall p1 p2,
+    asrt_to_list (p1 ** p2) = asrt_to_list p1 ++ asrt_to_list p2.
+Proof. 
+  intros.
+  unfold asrt_to_list.
+  generalize dependent p2.
+  induction p1; intros;
+    try solve [simpls; eauto]. 
+  -
+    assert (asrt_to_list' ((p1_1 ** p1_2) ** p2) [] =
+            asrt_to_list' (p1_1 ** p1_2 ** p2) []).
+    {
+      rewrite asrt_to_list'_assoc; eauto.
+    }
+    rewrite H.
+    rewrite IHp1_1; eauto.
+    rewrite IHp1_2; eauto.
+    rewrite IHp1_1; eauto.
+    rewrite app_assoc; eauto.
+Qed.
+
+Lemma FR_lst_to_asrt_app_stable1 :
+  forall l1 l2 rn,
+    FR rn (list_to_asrt l1) ->
+    FR rn (list_to_asrt (l1 ++ l2)).
+Proof.
+  intro l1.
+  induction l1; intros.
+  -
+    simpls; tryfalse.
+  -
+    simpl in H.
+    simpl.
+    destruct H; eauto.
+Qed.
+
+Lemma FR_lst_to_asrt_app_stable2 :
+  forall l1 l2 rn,
+    FR rn (list_to_asrt l2) ->
+    FR rn (list_to_asrt (l1 ++ l2)).
+Proof.
+  intro l1.
+  induction l1; intros.
+  -
+    simpls; eauto.
+  -
+    simpl.
+    eauto.
+Qed.
+
+Lemma FR_lst_to_asrt_app_stable_rev :
+  forall l1 l2 rn,
+    FR rn (list_to_asrt (l1 ++ l2)) ->
+    FR rn (list_to_asrt l1) \/ FR rn (list_to_asrt l2).
+Proof.
+  intro l1.
+  induction l1; intros.
+  -
+    simpls; eauto.
+  -
+    simpls.
+    destruct H; eauto.
+    eapply IHl1 in H.
+    destruct H; eauto.
+Qed.
+
+Lemma FReq_list_to_asrt_stable :
+  forall l1 l2,
+    FReq (list_to_asrt l1 ** list_to_asrt l2) (list_to_asrt (l1 ++ l2)).
+Proof.
+  intros.
+  unfolds FReq.
+  intro.
+  split.
+  {
+    intro.
+    simpls.
+    destruct H.
+    eapply FR_lst_to_asrt_app_stable1; eauto.
+    eapply FR_lst_to_asrt_app_stable2; eauto.
+  }
+  {
+    intro.
+    simpl.
+    eapply FR_lst_to_asrt_app_stable_rev; eauto.
+  }
+Qed.
+  
+Lemma list_asrt_app :
+  forall l1 l2 s,
+    s |= list_to_asrt l1 ** list_to_asrt l2 ->
+    s |= list_to_asrt (l1 ++ l2).
+Proof.
+  intro l1.
+  induction l1; intros.
+  -
+    simpls list_to_asrt.
+    eapply astar_emp_elim_l; eauto.
+  -
+    simpls list_to_asrt.
+    eapply astar_assoc_elim in H. 
+    eapply astar_subst2; eauto.
+    eapply FReq_list_to_asrt_stable; eauto.
+Qed.
+
+Lemma list_asrt_app_rev :
+  forall l1 l2 s,
+    s |= list_to_asrt (l1 ++ l2) ->
+    s |= list_to_asrt l1 ** list_to_asrt l2.
+Proof.
+  intro l1.
+  induction l1; intros.
+  -
+    simpls list_to_asrt.
+    eapply astar_emp_intro_l; eauto.
+  -
+    simpls list_to_asrt.
+    eapply astar_assoc_intro; eauto.
+    eapply astar_subst2; eauto.
+    eapply FReq_sym.
+    eapply FReq_list_to_asrt_stable; eauto.
+Qed.
+    
+Lemma l2a_a2l_stable' :
+  forall p1 p2 l1 l2 s,
+    s |= list_to_asrt (asrt_to_list' p1 l1) ** list_to_asrt (asrt_to_list' p2 l2) ->
+    s |= list_to_asrt (asrt_to_list' p1 l1 ++ asrt_to_list' p2 l2).
+Proof.
+  intro p1.
+  induction p1; intros;
+    simpl asrt_to_list' in *; simpl list_to_asrt in *;
+      try solve [eapply astar_assoc_elim in H; eapply astar_subst2; eauto;
+                try intros; eapply list_asrt_app; eauto].
+  -
+    eapply IHp1_1 in H; eauto.
+  -
+    eapply astar_assoc_elim in H0.
+    eapply astar_subst2; eauto.
+    intros.
+    eapply list_asrt_app; eauto.
+  -
+    eapply astar_assoc_elim in H0.
+    eapply astar_subst2; eauto.
+    intros.
+    eapply list_asrt_app; eauto.
+Qed.
+
+Lemma l2a_a2l_stable'_rev :
+  forall p1 p2 l1 l2 s,
+    s |= list_to_asrt (asrt_to_list' p1 l1 ++ asrt_to_list' p2 l2) ->
+    s |= list_to_asrt (asrt_to_list' p1 l1) ** list_to_asrt (asrt_to_list' p2 l2).
+Proof.
+  intro p1.
+  induction p1; intros;
+    simpl asrt_to_list' in *; simpl list_to_asrt in *;
+      try solve [eapply astar_assoc_intro; eapply astar_subst2; eauto;
+                 try intros; eapply list_asrt_app_rev; eauto].
+  eapply IHp1_1; eauto.
+Qed.
+    
+Lemma asrt_to_ls_stable :
+  forall p s,
+    s |= p ->
+    s |= list_to_asrt (asrt_to_list p).
+Proof.
+  intro p.
+  induction p; intros;
+    try solve [simpl list_to_asrt;
+               simpl asrt_to_list;
+               eapply astar_emp_intro_r; eauto].
+  eapply astar_subst1 in H; eauto.
+  eapply astar_subst2 in H; eauto.
+  rewrite asrt_to_list_app.
+  clear IHp1 IHp2.
+  unfolds asrt_to_list.
+  eapply l2a_a2l_stable'; eauto.
+Qed.
+
+Lemma asrt_to_ls_stable_rev :
+  forall p s,
+    s |= list_to_asrt (asrt_to_list p) ->
+    s |= p.
+Proof.
+  intro p.
+  induction p; intros;
+    try solve [simpls list_to_asrt; simpls asrt_to_list;
+               eapply astar_emp_elim_r; eauto].
+  eapply astar_subst1; eauto.
+  eapply astar_subst2; eauto.
+  rewrite asrt_to_list_app in H.
+  clear IHp1 IHp2.
+  unfolds asrt_to_list.
+  eapply l2a_a2l_stable'_rev; eauto.
+Qed.
+
+Ltac asrt_to_ls :=
+  match goal with
+  | |- _ |= _ =>
+    eapply asrt_to_ls_stable_rev;
+    simpl asrt_to_list; simpl list_to_asrt
+  | _ => idtac
+  end.
+
+Ltac asrt_to_ls_in H :=
+  match type of H with
+  | _ |= _ =>
+    eapply asrt_to_ls_stable in H;
+    simpl asrt_to_list in H; simpl list_to_asrt in H
+  | _ => idtac
+  end.
+
+Ltac sep_cancel1 m n :=
+  let H' := fresh in
+  match goal with
+  | H : ?s |= _ |- ?s |= _ =>
+    simpl_sep_liftn_in H m; simpl_sep_liftn n;
+    eapply astar_subst2; [eauto | introv H'; clear H]
+  | _ => idtac
+  end.
