coqimp/example/spec/spec.v
@@ -1,0 +1,77 @@
+Require Import Coqlib.        
+Require Import Maps.      
+Require Import LibTactics.  
+        
+Require Import Integers.  
+Open Scope Z_scope.     
+Import ListNotations.
+  
+Set Asymmetric Patterns.  
+       
+Require Import state.    
+Require Import language. 
+
+Set Implicit Arguments.  
+Unset Strict Implicit. 
+              
+Require Import logic.
+   
+Require Import lemmas.
+Require Import lemmas_ins.
+
+Require Import sep_lemma.
+Require Import reg_lemma.
+
+Require Import code.
+
+Require Import Coq.Logic.FunctionalExtensionality.
+  
+Open Scope nat.
+Open Scope code_scope.
+Open Scope mem_scope.
+
+(** Some auxiliary definition *)
+Definition winvalid x y :=
+  win_masked x y = false.
+
+(** Specification *)
+Definition add_pre (vl : list logicvar) :=
+  EX x y z w fret,
+  [| vl = logic_lv x :: logic_lv y :: logic_lv z :: logic_lv fret :: nil |] **
+  i0 |=> x ** i1 |=> y ** i2 |=> z ** l7 |=> w ** r15 |=> fret.
+
+Definition add_post (vl : list logicvar) :=
+  EX x y z fret,
+  [| vl = logic_lv x :: logic_lv y :: logic_lv z :: logic_lv fret :: nil |] **
+  i0 |=> x ** i1 |=> y ** i2 |=> z ** l7 |=> (x +ᵢ y +ᵢ z) ** r15 |=> fret.
+
+Definition changeY_pre (vl : list logicvar) :=
+  EX fmo fml fmi fret x vy vi id fm1 fm2 F,
+  [| vl = logic_fm fmi :: logic_fm fm1 :: logic_fm fm2
+          :: logic_lv x :: logic_lv fret :: logic_lv vy :: logic_lv vi :: nil |] **
+  Regs fmo fml fmi ** Ry |=> vy ** Rwim |=> vi ** {| id, fm1 :: fm2 :: F |} **
+  [| get_frame_nth fmi 7 = Some fret /\ get_frame_nth fmi 0 = Some x
+     /\ winvalid (post_cwp id) vi |].
+
+Definition changeY_post (vl : list logicvar) :=
+  EX fmo fml fmi fret x vy vi id fm1 fm2 F,
+  [| vl = logic_fm fmi :: logic_fm fm1 :: logic_fm fm2
+          :: logic_lv x :: logic_lv fret :: logic_lv vy :: logic_lv vi :: nil |] **
+  Regs (update_frame fmi 0 vy) fm1 fm2 ** Ry |=> vy ** Ry |=> x ** Rwim |=> vi **
+  {| post_cwp id, F ++ (fmo :: fml :: nil) |}.
+
+Fixpoint convert_spec (ls : list (Address * fspec)) :
+  funspec :=
+  match ls with
+  | nil => fun _ : Address => None
+  | (f', spec) :: ls' =>
+    fun f : Address =>
+      if AddrEq.eq f f' then
+        Some spec
+      else
+        convert_spec ls' f
+  end.
+
+
+
+  
