coqimp/framework/soundness/wfcdhp_sound.v
@@ -64,42 +64,6 @@ Proof.
   subst.
   eauto.
 Qed.
-
-Lemma pc_jmpl_npc_i_or_jmp :
-  forall pc npc C aexp1 r1 I,
-    LookupC C pc npc I ->
-    C pc = Some (cjumpl aexp1 r1) ->
-    (exists i, C npc = Some (cntrans i)) \/ (exists aexp2 r2, C npc = Some (cjumpl aexp2 r2)).
-Proof.
-  intros.
-  inversion H; get_ins_diff_false.
-  left.
-  eauto.
-  right.
-  eauto.
-Qed.
-
-Lemma pc_be_npc_i :
-  forall pc npc C aexp I,
-    LookupC C pc npc I ->
-    C pc = Some (cbe aexp) ->
-    exists i, C npc = Some (cntrans i).
-Proof.
-  intros.
-  inversion H; get_ins_diff_false.
-  eauto.
-Qed.
-
-Lemma pc_bne_npc_i :
-  forall pc npc C aexp I,
-    LookupC C pc npc I ->
-    C pc = Some (cbne aexp) ->
-    exists i, C npc = Some (cntrans i).
-Proof.
-  intros.
-  inversion H; get_ins_diff_false.
-  eauto.
-Qed.
   
 (*+ Well-formed function proof +*)
 Lemma safety_Sn_safety_n :
@@ -192,7 +156,7 @@ Proof.
   -
     econstructor; eauto.
 
-  -
+  - 
     inversion H; subst.
 
     + 
@@ -238,17 +202,14 @@ Proof.
       simpls.
       simpljoin1.
       simpls.
-      eapply H13 in H7; eauto.
+      eapply H13 in H; eauto.
       simpls.
       simpljoin1.
       rewrite get_R_rn_neq_r0; eauto.
       2 : intro; tryfalse.
-      rewrite get_R_rn_neq_r0 in H3; eauto.
+      rewrite get_R_rn_neq_r0 in H; eauto.
       2 : intro; tryfalse.
-      rewrite get_R_rn_neq_r0 in H4; eauto.
-      2 : intro; tryfalse.
-      unfold merge.
-      rewrite H4; eauto.
+      eapply disj_in_m1_merge_still; eauto.
       intros.
       eapply IHn; eauto.
       intros.
@@ -440,26 +401,18 @@ Proof.
       eapply wf_seq_frame_rule in H6; eauto.
       unfolds insSeq_sound.
       eapply H6; eauto.
-      simpl.
+      simpl. 
       exists (m, (r0, f1), d0) (m0, (r1, f1), d0).
-      repeat (split; eauto).
-      intros.
-      clear - H9 H6 H12.
+      repeat (split; eauto). 
+      intros. 
+      clear - H6 H12.
       sep_star_split_tac.
       simpls.
       simpljoin1.
       simpls.
-      eapply H12 in H; eauto.
+      eapply H12 in H1; eauto.
       simpls.
-      simpljoin1.
-      rewrite get_R_rn_neq_r0; eauto.
-      2 : intro; tryfalse.
-      rewrite get_R_rn_neq_r0 in H; eauto.
-      2 : intro; tryfalse.
-      rewrite get_R_rn_neq_r0 in H5; eauto.
-      2 : intro; tryfalse.
-      unfold merge. 
-      rewrite H5; eauto. 
+      eapply get_R_merge_still; eauto.
 
     +
       econstructor; intros; get_ins_diff_false.
@@ -614,14 +567,14 @@ Proof.
       left.
       simpljoin1.
       eauto.
-Qed.  
+Qed.
 
 (** wf_function means if the current instruction sequence is well-formed and the code heap is well-formed, then we get the execution of the current function is safe for any steps n *)
 Theorem wf_function :
-  forall p q Spec Spec' S C pc npc I,
-    insSeq_sound Spec p I q -> LookupC C pc npc I ->
+  forall p q Spec Spec' S C pc I,
+    insSeq_sound Spec p pc I q -> LookupC C pc I ->
     cdhp_subst Spec Spec' -> cdhp_sound Spec C Spec' -> S |= p ->
-    forall n, safety n C S pc npc q 0.
+    forall n, safety n C S pc (pc +ᵢ ($ 4)) q 0.
 Proof.
   intros.
   unfolds insSeq_sound.
